WIP: Export code

Ground_PDDL_Exec_Imp/Check_Unsolvability.thy
@@ -5,19 +5,6 @@ theory Check_Unsolvability
     Munta_Certificate_Checker.Simple_Network_Language_Certificate_Code
 begin
 
-
-fun act_sym'  where
-"act_sym' (In a) = a" |
-"act_sym' (Out a) = a" |
-"act_sym' (Sil a) = a"
-
-declare act_sym'.simps[code del]
-
-
-
-code_thms act_sym'
-
-
 fun act_sym where
 "act_sym (In a) = a" |
 "act_sym (Out a) = a" |
@@ -37,10 +24,10 @@ definition action_list where
 declare Simple_Network_Impl.action_set_def[code del]
 
 lemma [code]: "Simple_Network_Impl.action_set = (\<lambda>automata broadcast. action_list automata broadcast |> set)"
-  sorry
+  sorry                               
 
 
-definition "clkp_list' automata =
+definition "clkp_set_impl automata =
 automata
 |> map (\<lambda>A. snd (snd (snd A)))
 |> map (map (\<lambda>(l, invs). invs))
@@ -49,9 +36,9 @@ automata
 |> foldl (\<union>) {}"
 
 
-definition "clk_list' automata = 
+definition "clk_set_impl automata = 
 (automata 
-|> clkp_list'
+|> clkp_set_impl
 |> (`) fst)
 \<union> (
 automata
@@ -60,27 +47,34 @@ automata
 |> foldl (@) []
 |> foldl (\<union>) {})"
 
+lemma trans_refine:
+  "(\<Union>(l, e, g, a, r, u, l')\<in>Simple_Network_Language.trans (Simple_Network_Language.Prod_TA_Defs.N (set broadcast, map automaton_of automata, map_of bounds') i). {l, l'}) = 
+  (automata ! i
+  |> (\<lambda>(_,_,ts,_). ts)
+  |> map (\<lambda>(l, _, _, _, _, _, l'). {l, l'})
+  |> foldl (\<union>) {}
+  )"
+  sorry
 
 
 declare Simple_Network_Impl.clk_set'_def[code del] 
 
-(* Don't use List.list.set here. Circular dependency. Need to use set_aux (of_phantom set_impl) *)
-lemma [code]: "Simple_Network_Impl.clk_set' = (\<lambda>automata. clk_list' automata)"
+lemma [code]: "Simple_Network_Impl.clk_set' = (\<lambda>automata. clk_set_impl automata)"
   sorry
 
-definition "loc_list' automata p \<equiv>
+definition "loc_set_impl automata p \<equiv>
 (fst (snd (snd (automata ! p))))
 |> map (\<lambda>(l, _, _, _, _, _, l'). {l, l'})
 |> foldl (\<union>) {}"
 
 declare Simple_Network_Impl.loc_set'_def[code del]
 
-lemma [code]: "Simple_Network_Impl.loc_set' = (\<lambda>automata p. loc_list' automata p)"
+lemma [code]: "Simple_Network_Impl.loc_set' = (\<lambda>automata p. loc_set_impl automata p)"
   sorry
 
 
-fun loc_list where
-"loc_list (broadcast, automata, bounds) = 
+fun prod_TA_loc_set_impl where
+"prod_TA_loc_set_impl (broadcast, automata, bounds) = 
 (
 let trans = [0..<length automata] 
     |> (map (\<lambda>p. automata ! p |> (\<lambda>(_, _, trans,_). trans)));
@@ -91,17 +85,20 @@ let trans = [0..<length automata]
 in locs
 )"
 
-
-declare Prod_TA_Defs.var_set_def[code del]
+(* It's better not to declare these deleted.
+If they are deleted, they will throw an error during runtime.
+If not, any export that refers to them will throw an error
+declare Prod_TA_Defs.loc_set_def[code del] *)
 
 lemma loc_set_alt:
   "Prod_TA_Defs.loc_set (set broadcast, map automaton_of automata, map_of bounds) = 
-    loc_list (broadcast, automata, bounds)"
+    prod_TA_loc_set_impl (broadcast, automata, bounds)"
   sorry
 
 
-fun var_set where
-"var_set (broadcast, automata, bounds) = 
+
+fun prop_TA_var_set_impl where
+"prop_TA_var_set_impl (broadcast, automata, bounds) = 
 ([0..<length automata]
 |> (map (\<lambda>p. automata ! p |> (\<lambda>(_, _, trans,_). trans)))
 |> (map (map (\<lambda>(_, b, _, _, _, _, _). b)))
@@ -117,21 +114,31 @@ fun var_set where
 |> foldl (@) []
 |> foldl (\<union>) {}) "
 
-declare Prod_TA_Defs.var_set_def[code del]
+(* declare Prod_TA_Defs.var_set_def[code del] *)
 
 lemma var_set_alt:
   "Prod_TA_Defs.var_set (set broadcast, map automaton_of automata, map_of bounds) 
-    = var_set (broadcast, automata, bounds)"
+    = prop_TA_var_set_impl (broadcast, automata, bounds)"
   sorry
 
 
-fun act_set where
-"act_set (broadcast, automata, bounds) =
-undefined"
+fun prod_TA_act_set_impl where
+"prod_TA_act_set_impl (broadcast, automata, bounds) =
+([0..<length automata]
+|> (map (\<lambda>p. automata ! p |> (\<lambda>(_, _, trans,_). trans)))
+|> (map (map (\<lambda>(_, _, _, a, _, _, _). set_act a)))
+|> foldl (@) []
+|> foldl (\<union>) {}
+)
+\<union>
+set broadcast"
+
+(* declare Prod_TA_Defs.act_set_def[code del] *)
 
 lemma act_set_alt:
   "Prod_TA_Defs.act_set (set broadcast, map automaton_of automata, map_of bounds)
-    = act_set (broadcast, automata, bounds)" sorry
+    = prod_TA_act_set_impl (broadcast, automata, bounds)" sorry
+
 
 derive (eq) ceq bexp act acconstraint exp
 
@@ -145,41 +152,6 @@ derive (rbt) set_impl act acconstraint
 derive (no) ccompare exp bexp
 
 
-(* definition "make_renaming \<equiv> \<lambda> broadcast automata bounds.
-  let
-    action_set = Simple_Network_Impl.action_set automata broadcast |> list_of_set;
-    clk_set = Simple_Network_Impl.clk_set' automata |> list_of_set;
-    clk_set = clk_set @ [STR ''_urge''];
-    loc_set' = (\<lambda>i. Simple_Network_Impl.loc_set' automata i |> list_of_set);
-    loc_set = Prod_TA_Defs.loc_set
-      (set broadcast, map automaton_of automata, map_of bounds);
-    loc_set_diff = (\<lambda>i. loc_set - Simple_Network_Impl.loc_set' automata i |> list_of_set);
-    loc_set = list_of_set loc_set;
-    var_set = Prod_TA_Defs.var_set
-      (set broadcast, map automaton_of automata, map_of bounds) |> list_of_set;
-    n_ps = length automata;
-    num_actions = length action_set;
-    m = length (remdups clk_set);
-    num_states_list = map (\<lambda>i. loc_set' i |> remdups |> length) [0..<n_ps];
-    num_states = (\<lambda>i. num_states_list ! i);
-    mk_renaming = mk_renaming (\<lambda>x. x)
-  in do {
-    ((renum_acts, _), (renum_clocks, inv_renum_clocks), (renum_vars, inv_renum_vars)) \<leftarrow>
-      mk_renaming action_set <|> mk_renaming clk_set <|> mk_renaming var_set;
-    let renum_clocks = Suc o renum_clocks;
-    let inv_renum_clocks = (\<lambda>c. if c = 0 then STR ''0'' else inv_renum_clocks (c - 1));
-    renum_states_list' \<leftarrow> combine_map (\<lambda>i. mk_renaming' (loc_set' i)) [0..<n_ps];
-    let renum_states_list = map fst renum_states_list';
-    let renum_states_list = map_index
-      (\<lambda>i m. extend_domain m (loc_set_diff i) (length (loc_set' i))) renum_states_list;
-    let renum_states = (\<lambda>i. renum_states_list ! i);
-    let inv_renum_states = (\<lambda>i. map snd renum_states_list' ! i);
-    assert (fst ` set bounds \<subseteq> set var_set)
-      STR ''State variables are declared but do not appear in model'';
-    Result (m, num_states, num_actions, renum_acts, renum_vars, renum_clocks, renum_states,
-      inv_renum_states, inv_renum_vars, inv_renum_clocks)
-  }" *)
-
 declare make_renaming_def[code del]
 
 
@@ -190,8 +162,98 @@ schematic_goal make_renaming'[code]: "make_renaming \<equiv> ?x"
   unfolding loc_set_alt
   ..
 
-export_code make_renaming
-  in Eval module_name make_renaming file_prefix Test
+(* Circular dependency error resolved by providing a module name ... *)
+
+declare Simple_Network_Impl_nat_defs.clkp_set''_def[code del]
+
+definition "clkp_set''_impl automata i l \<equiv> 
+Simple_Network_Impl_nat_defs.clkp_inv automata i l \<union> 
+(automata ! i
+|> (\<lambda>a. fst (snd (snd a)))
+|> map (\<lambda>(l', b, g, _). if l' = l then collect_clock_pairs g else {})
+|> foldl (\<union>) {})"
+
+lemma [code]: "Simple_Network_Impl_nat_defs.clkp_set'' = clkp_set''_impl"
+  sorry
+
+lemma set_foldl_append: "(set (foldl (@) xs ys)) = \<Union>(set ` (insert xs (set ys)))"
+  apply (induction ys arbitrary: xs)
+  by auto
+
+lemma invs_refine: "\<Union> ((\<lambda>g. fst ` set g) ` set (map (snd o snd o snd) automata)) =
+  automata
+  |> map (\<lambda>(committed, urgent, trans, invs). invs)
+  |> map (map (\<lambda>(loc, inv). loc))
+  |> foldl (@) []
+  |> set"
+  unfolding image_set
+  unfolding map_map
+  unfolding comp_def
+  unfolding set_foldl_append
+  by force
+
+schematic_goal in_states_refine: "L \<in> Prod_TA_Defs.states (set broadcast, map automaton_of automata, map_of bounds')
+  = ?x"
+  unfolding Prod_TA_Defs.states_def
+  unfolding mem_Collect_eq
+  unfolding trans_refine 
+  ..
+
+thm Simple_Network_Rename_Formula_String_Defs.check_renaming_def[no_vars]
+
+thm Simple_Network_Rename_Formula_String_Defs.check_renaming_def
+
+declare Simple_Network_Rename_Formula_String_Defs.check_renaming_def[code del]
+
+schematic_goal check_renaming_imp[code]: "Simple_Network_Rename_Formula_String_Defs.check_renaming = ?x"
+  unfolding Simple_Network_Rename_Formula_String_Defs.check_renaming_def
+  unfolding var_set_alt loc_set_alt act_set_alt
+  unfolding image_set
+  unfolding invs_refine
+  unfolding in_states_refine
+  ..
+
+declare Simple_Network_Impl_nat_defs.check_precond2_def[code del]
+
+schematic_goal check_precond2_impl[code]: "Simple_Network_Impl_nat_defs.check_precond2 = ?x"
+  unfolding Simple_Network_Impl_nat_defs.check_precond2_def
+  unfolding list_all_iff[symmetric]
+  unfolding image_set
+  unfolding Simple_Network_Impl_Defs.n_vs_def
+  unfolding Prod_TA_Defs.n_ps_def
+  unfolding Prod_TA_Defs.bounds_def (* Some of these constants have no definitions *)
+  unfolding prod.case fst_conv snd_conv length_map
+  ..
+
+
+(* export_code Simple_Network_Impl_nat_defs.check_precond2
+  in Eval module_name check_precond_2_test file_prefix x *)
+
+declare Simple_Network_Impl_nat_ceiling_start_state_axioms_def[code del]
+
+schematic_goal nat_ceiling_start_state_axioms_impl[code]: "Simple_Network_Impl_nat_ceiling_start_state_axioms = ?x"
+  unfolding Simple_Network_Impl_nat_ceiling_start_state_axioms_def
+  unfolding list_all_iff[symmetric]
+  unfolding Simple_Network_Impl_Defs.n_vs_def
+  unfolding Prod_TA_Defs.n_ps_def
+  unfolding Prod_TA_Defs.bounds_def
+  unfolding image_set
+  unfolding prod.case fst_conv snd_conv length_map
+  ..
+
+thm Simple_Network_Impl_nat_defs.states_i_def
+declare Simple_Network_Impl_nat_defs.states_i_def[code del]
+
+schematic_goal states_i_impl[code]: "Simple_Network_Impl_nat_defs.states_i = ?x"
+  unfolding Simple_Network_Impl_nat_defs.states_i_def
+  unfolding list_all_iff[symmetric]
+  unfolding Simple_Network_Impl_Defs.n_vs_def
+  unfolding Prod_TA_Defs.n_ps_def
+  unfolding Prod_TA_Defs.bounds_def
+  unfolding image_set
+  unfolding prod.case fst_conv snd_conv length_map
+  ..
+
 
 
 definition compute_model::"
@@ -265,22 +327,6 @@ definition compute_model::"
           inv_renum_states, inv_renum_vars, inv_renum_clocks)
    }"
 
-declare Simple_Network_Impl_nat_defs.clkp_set''_def[code del]
-
-definition "clkp_set''_impl automata i l \<equiv> 
-Simple_Network_Impl_nat_defs.clkp_inv automata i l \<union> 
-(automata ! i
-|> (\<lambda>a. fst (snd (snd a)))
-|> map (\<lambda>(l', b, g, _). if l' = l then collect_clock_pairs g else {})
-|> foldl (\<union>) {})"
-
-lemma x[code]: "Simple_Network_Impl_nat_defs.clkp_set'' = clkp_set''_impl"
-  sorry
-
-(* 
-export_code compute_model
-  in Eval module_name make_renaming file_prefix 1234 *)
-
 
 definition "certificate_check" where
 "certificate_check mode num_split dc state_space broadcast bounds automata k L\<^sub>0 s\<^sub>0 formula
@@ -306,6 +352,9 @@ definition "certificate_check" where
       (buechi_of state_space) |> Heap_Monad.return
 }
 " for num_split and state_space :: "nat state_space"
+
+(* export_code certificate_check
+  in Eval module_name make_renaming file_prefix Test *)
 
 lemma certificate_check_okay: 
   fixes num_split state_space
@@ -420,6 +469,34 @@ of Result c \<Rightarrow> do {
 | Error es \<Rightarrow> Heap_Monad.return (Error es))
 " for num_split and state_space :: "int state_space"
 
+find_theorems name: "Error_List*case"
+
+thm return_cons_rule
+
+find_theorems "?P \<Longrightarrow>\<^sub>A ?R ?x"
+
+thm return_cons_rule
+
+(* This made things really hard *)
+lemma Error_List_Monad_result_case_rule:
+  assumes "\<And>x. result = Result x \<Longrightarrow> <P> Heap_Monad.return x <R>"
+          "\<And>x. <R x> f1 x <Q>" 
+      and "\<And>x. result = Error x \<Longrightarrow> <P> Heap_Monad.return x <S>"
+          "\<And>x. <S x> f2 x <Q>" 
+  shows "<P> (case result of Result x \<Rightarrow> f1 x | Error x \<Rightarrow> f2 x) <Q>"
+  apply (cases result)
+   apply (rule ssubst, assumption)
+   apply (subst Error_List_Monad.result.case)
+   apply (rule Hoare_Triple.cons_pre_rule[OF _ assms(2)])
+   apply (frule assms(1)) 
+  apply (erule Unreachability_Misc.return_htD)
+   apply (rule ssubst, assumption)
+   apply (subst Error_List_Monad.result.case)
+  apply (rule Hoare_Triple.cons_pre_rule[OF _ assms(4)])
+   apply (frule assms(3)) 
+  by (erule Unreachability_Misc.return_htD)
+
+
 lemma convert_check_okay:
   fixes num_split state_space
   assumes mode: "mode \<noteq> Buechi" "mode \<noteq> Debug"
@@ -443,8 +520,8 @@ proof (cases "make_renaming broadcast automata bounds")
   obtain aa ba ca da ea fa g where
     x1: "x1 = (aa, ba, ca, da, ea, fa, g)" by (cases x1) auto
 
-  obtain renum_states uu  uua  uub where
-    g: "g = (renum_states, uu, uua, uub)" by (cases g) auto
+  obtain renum_states renum_vars x y where
+    g: "g = (renum_states, renum_vars, x, y)" by (cases g) auto
 
   obtain broadcast' automata' bounds' where
     rename: "rename_network broadcast bounds automata da a b c = (broadcast', automata', bounds')" 
@@ -535,6 +612,93 @@ next
     unfolding Error_List_Monad.result.case
     by auto
 qed
+(* Hoare Logic is tedious in this case
+  unfolding convert_check_def
+proof (rule Error_List_Monad_result_case_rule)
+  fix c
+  assume comp: "compute_model model renaming \<bind>
+         (\<lambda>r. let (broadcast, bounds, automata, urgent_locations, k, L\<^sub>0, s\<^sub>0, formula, m, num_states, num_actions, renum_acts, renum_vars, renum_clocks, renum_states, inv_renum_states, inv_renum_vars,
+                     inv_renum_clocks) = r;
+                   is_urgent = \<lambda>(L, L'). list_ex (\<lambda>(l, urgent). l \<in> set urgent) (zip L (map (map int) urgent_locations)); inv_renum_clocks = \<lambda>i. if i = m then STR ''_urge'' else inv_renum_clocks i; t = now ();
+                   state_space = convert_state_space m is_urgent state_space; t = now () - t; _ = println (STR ''Time for converting state space: '' + time_to_string t); _ = start_timer ();
+                   _ = save_time STR ''Time for converting DBMs in certificate''; _ = println (STR ''Number of discrete states: '' + show_lit (len_of_state_space state_space));
+                   _ = if show_cert
+                       then let _ = print_sep (); _ = println STR ''Certificate''; _ = print_sep (); _ = show_state_space m inv_renum_states inv_renum_vars inv_renum_clocks state_space; _ = print_sep ()
+                            in Heap_Monad.return ()
+                       else Heap_Monad.return ()
+               in Result
+                   (certificate_check mode num_split False state_space broadcast bounds automata k L\<^sub>0 s\<^sub>0 formula m num_states num_actions renum_acts renum_vars renum_clocks renum_states inv_renum_states
+                     inv_renum_vars inv_renum_clocks)) =
+         Result c"
+  show "<emp> Heap_Monad.return c <\<lambda>c. \<up>(\<exists>state_space broadcast bounds automata k L\<^sub>0 s\<^sub>0 formula m num_states num_actions renum_acts renum_vars renum_clocks renum_states (inv_renum_states::nat \<Rightarrow> nat \<Rightarrow> nat)
+                     (inv_renum_vars::nat \<Rightarrow> String.literal) (inv_renum_clocks::nat \<Rightarrow> String.literal). c = certificate_check mode num_split False state_space broadcast bounds automata k L\<^sub>0 s\<^sub>0 formula m num_states num_actions renum_acts renum_vars renum_clocks renum_states inv_renum_states
+                     inv_renum_vars inv_renum_clocks)>"
+  proof (cases "compute_model model renaming")
+    case res1: (Result x1)
+    
+    show ?thesis
+    proof (cases x1)
+      case x1: (fields a1 b1 c1 d1 e1 f1 g1)
+      show ?thesis
+      proof (cases g1)
+        case g1: (fields a2 b2 c2 d2 e2 f2 g2)
+        show ?thesis 
+        proof (cases g2)
+          case g2: (fields a3 b3 c3 d3 e3 f3)
+          have c: "c =  (certificate_check mode num_split False (convert_state_space c2 (\<lambda>(L, L'). list_ex (\<lambda>(l, urgent). l \<in> set urgent) (zip L (map (map int) d1))) state_space) a1 b1 c1 e1 f1 a2 b2 c2 d2 e2 f2 a3 b3 c3 d3 e3
+             (\<lambda>i. if i = c2 then STR ''_urge'' else f3 i))"
+            using comp unfolding res1 x1 g1 g2 bind.simps Let_def Error_List_Monad.result.case prod.case by auto
+          show ?thesis 
+            unfolding c
+            apply (rule return_cons_rule)
+            by fastforce
+        qed
+      qed
+    qed
+  next
+    case err1: (Error x2)
+    show ?thesis using comp unfolding err1 bind.simps Let_def Error_List_Monad.result.case by auto
+  qed
+next
+  fix c
+  show "<\<up> (\<exists>state_space broadcast bounds automata k m num_states num_actions renum_acts renum_vars renum_clocks renum_states inv_renum_states inv_renum_vars inv_renum_clocks.
+                c =
+                certificate_check mode num_split False state_space broadcast bounds automata k L\<^sub>0 s\<^sub>0 formula m num_states num_actions renum_acts renum_vars renum_clocks renum_states inv_renum_states inv_renum_vars
+                 inv_renum_clocks)> let t = now ()
+                                    in c \<bind>
+                                       (\<lambda>check.
+                                           let _ = case check of Renaming_Failed \<Rightarrow> let _ = println STR ''Renaming failed'' in Heap_Monad.return ()
+                                                   | Preconds_Unsat \<Rightarrow> let _ = println STR ''Preconditions were not met'' in Heap_Monad.return ()
+                                                   | Sat \<Rightarrow> let _ = println STR ''Certificate was accepted'' in Heap_Monad.return ()
+                                                   | Unsat \<Rightarrow> let _ = println STR ''Certificate was rejected'' in Heap_Monad.return ();
+                                               t = now () - t; _ = println (STR ''Time for certificate checking: '' + time_to_string t)
+                                           in Heap_Monad.return
+                                               (Result
+                                                 check)) <\<lambda>r. case r of Result Sat \<Rightarrow> \<up> (\<not> Simple_Network_Language_Model_Checking.N broadcast automata bounds,(L\<^sub>0, map_of s\<^sub>0, \<lambda>_. 0) \<Turnstile> formula) | Result _ \<Rightarrow> true
+                                                               | Error e \<Rightarrow> true>\<^sub>t"
+  proof (rule Hoare_Triple.norm_pre_pure_rule2)
+    assume "\<exists>state_space broadcast bounds automata k L\<^sub>0 s\<^sub>0 formula m num_states num_actions renum_acts renum_vars renum_clocks renum_states (inv_renum_states::nat \<Rightarrow> nat \<Rightarrow> nat)
+                     (inv_renum_vars::nat \<Rightarrow> String.literal) (inv_renum_clocks::nat \<Rightarrow> String.literal).
+       c =
+       certificate_check mode num_split False state_space broadcast bounds automata k L\<^sub>0 s\<^sub>0 formula m num_states num_actions renum_acts renum_vars renum_clocks renum_states inv_renum_states inv_renum_vars
+        inv_renum_clocks"
+    then obtain state_space broadcast' bounds' automata' k  m num_states num_actions renum_acts renum_vars renum_clocks and renum_states inv_renum_states::"nat \<Rightarrow> nat \<Rightarrow> nat" and inv_renum_vars::"nat \<Rightarrow> String.literal" and inv_renum_clocks::"nat \<Rightarrow> String.literal" where
+    c: "c =
+       certificate_check mode num_split False state_space broadcast bounds automata k L\<^sub>0 s\<^sub>0 formula m num_states num_actions renum_acts renum_vars renum_clocks renum_states inv_renum_states inv_renum_vars
+        inv_renum_clocks"  by blast
+    show " <emp> let t = now ()
+          in c \<bind>
+             (\<lambda>check.
+                 let _ = case check of Renaming_Failed \<Rightarrow> let _ = println STR ''Renaming failed'' in Heap_Monad.return ()
+                         | Preconds_Unsat \<Rightarrow> let _ = println STR ''Preconditions were not met'' in Heap_Monad.return () | Sat \<Rightarrow> let _ = println STR ''Certificate was accepted'' in Heap_Monad.return ()
+                         | Unsat \<Rightarrow> let _ = println STR ''Certificate was rejected'' in Heap_Monad.return ();
+                     t = now () - t; _ = println (STR ''Time for certificate checking: '' + time_to_string t)
+                 in Heap_Monad.return
+                     (Result check)) <\<lambda>r. case r of Result Sat \<Rightarrow> \<up> (\<not> Simple_Network_Language_Model_Checking.N broadcast automata bounds,(L\<^sub>0, map_of s\<^sub>0, \<lambda>_. 0) \<Turnstile> formula) | Result _ \<Rightarrow> true | Error e \<Rightarrow> true>\<^sub>t"
+      
+  qed
+qed
+*)
 
 instantiation predicate::"show"
 begin
@@ -572,23 +736,6 @@ instance
   done
 end
 
-
-(* Need a function that can be called with the computed certificate and renaming *)
-
-(* To do:
-  - Write a function, which checks all the conditions of the locale.
-  - Do the functions implemented in the locale need to be re-implemented for executability?
-  - Which names do we need to pass here?
-*)
-
-thm Simple_Network_Rename_Formula_String_Defs.check_renaming_def
-
-schematic_goal [code]: "Simple_Network_Rename_Formula_String_Defs.check_renaming = ?x"
-  unfolding Simple_Network_Rename_Formula_String_Defs.check_renaming_def
-  unfolding var_set_alt loc_set_alt
-
-export_code Simple_Network_Rename_Formula_String_Defs.check_renaming
-  in Eval module_name convert_check file_prefix 1234 
 
 (* The certifier takes a list of names clocks and automata, 
   which it would otherwise obtain when parsing *)
@@ -751,16 +898,7 @@ do {
 " for num_split
 
 
-thm Simple_Network_Rename_Formula_String_Defs.check_renaming_def[no_vars]
-
-export_code Simple_Network_Impl.clk_set'
-
-declare Simple_Network_Impl.clk_set'_def[code del]
-
-export_code Simple_Network_Rename_Formula_String_Defs.check_renaming
-
-
-export_code check_and_cert_pddl_problem
+export_code check_and_cert_pddl_problem_no_return
   in Eval module_name Certifier file_prefix certifier
 (* To do:
   - Change the parser for PDDL. (ML)
